ZKLib/OracleReduction/Basic.lean
@@ -267,89 +267,6 @@ instance {pSpec : ProtocolSpec n} {oSpec : OracleSpec ι} {PrvState : Type}
 
 end Format
 
-section Restrict
-
-variable {n : ℕ}
-
-abbrev ProtocolSpec.take (m : ℕ) (h : m ≤ n) (pSpec : ProtocolSpec n) :=
-  Fin.take m h pSpec
-
-abbrev ProtocolSpec.rtake (m : ℕ) (h : m ≤ n) (pSpec : ProtocolSpec n) :=
-  Fin.rtake m h pSpec
-
-abbrev Transcript.take {pSpec : ProtocolSpec n} (m : ℕ) (h : m ≤ n)
-    (transcript : Transcript pSpec) : Transcript (pSpec.take m h) :=
-  Fin.take m h transcript
-
-abbrev Transcript.rtake {pSpec : ProtocolSpec n} (m : ℕ) (h : m ≤ n)
-    (transcript : Transcript pSpec) : Transcript (pSpec.rtake m h) :=
-  Fin.rtake m h transcript
-
-end Restrict
-
-section Composition
-
-variable {n m : ℕ}
-
-/-- Adding a round with direction `dir` and type `Message` to the beginning of a `ProtocolSpec` -/
-abbrev ProtocolSpec.cons (pSpec : ProtocolSpec n) (dir : Direction) (Message : Type) :
-    ProtocolSpec (n + 1) :=
-  Fin.cons ⟨dir, Message⟩ pSpec
-
-/-- Adding a round with direction `dir` and type `Message` to the end of a `ProtocolSpec` -/
-abbrev ProtocolSpec.snoc (pSpec : ProtocolSpec n) (dir : Direction) (Message : Type) :
-    ProtocolSpec (n + 1) :=
-  Fin.snoc pSpec ⟨dir, Message⟩
-
-/-- Appending two `ProtocolSpec`s -/
-abbrev ProtocolSpec.append (pSpec : ProtocolSpec n) (pSpec' : ProtocolSpec m) :
-    ProtocolSpec (n + m) :=
-  Fin.append pSpec pSpec'
-
-def ProtocolSpec.mkSingle (dir : Direction) (Message : Type) : ProtocolSpec 1 :=
-  fun _ => ⟨dir, Message⟩
-
-infixl : 65 " ++ₚ " => ProtocolSpec.append
-
-@[simp]
-theorem ProtocolSpec.snoc_take {pSpec : ProtocolSpec n} (m : ℕ) (h : m < n) :
-    (pSpec.take m (by omega) ++ₚ (fun (_ : Fin 1) => pSpec ⟨m, h⟩))
-        = pSpec.take (m + 1) (by omega) := by
-  simp only [append, take, Fin.append_right_eq_snoc, Fin.take_succ_eq_snoc]
-
-/-- Appending two `ToOracle`s for two `ProtocolSpec`s -/
-def ToOracle.append {pSpec₁ : ProtocolSpec n} {pSpec₂ : ProtocolSpec m}
-    [O₁ : ∀ i, ToOracle (pSpec₁.Message i)] [O₂ : ∀ i, ToOracle (pSpec₂.Message i)] :
-        ∀ i, ToOracle ((pSpec₁ ++ₚ pSpec₂).Message i) := fun ⟨i, h⟩ => by
-  dsimp [ProtocolSpec.append, ProtocolSpec.getDir] at h ⊢
-  dsimp [ProtocolSpec.Message, ProtocolSpec.getType]
-  by_cases h' : i < n
-  · rw [← Fin.castAdd_castLT m i h', Fin.append_left] at h ⊢
-    exact O₁ ⟨i.castLT h', h⟩
-  · rw [← @Fin.natAdd_subNat_cast n m i (not_lt.mp h'), Fin.append_right] at h ⊢
-    exact O₂ ⟨Fin.subNat n (Fin.cast (add_comm n m) i) (not_lt.mp h'), h⟩
-
-instance {pSpec : ProtocolSpec n} {pSpec' : ProtocolSpec m}
-    [∀ i, ToOracle (pSpec.Message i)] [∀ i, ToOracle (pSpec'.Message i)] :
-    ∀ i, ToOracle ((pSpec ++ₚ pSpec').Message i) := ToOracle.append
-
-/-- Appending two transcripts for two `ProtocolSpec`s -/
-def Transcript.append {pSpec₁ : ProtocolSpec n} {pSpec₂ : ProtocolSpec m}
-    (T₁ : Transcript pSpec₁) (T₂ : Transcript pSpec₂) : Transcript (pSpec₁ ++ₚ pSpec₂) := by
-  dsimp [ProtocolSpec.append, ProtocolSpec.getDir]
-  dsimp [Transcript, ProtocolSpec.getType] at T₁ T₂ ⊢
-  exact fun i => (Fin.append_comp Prod.snd i) ▸ (Fin.addCases' T₁ T₂ i)
-
-infixl : 65 " ++ₜ " => Transcript.append
-
-/-- Adding a message with a given direction and type to the end of a `Transcript` -/
-def Transcript.snoc {pSpec : ProtocolSpec n} {NextMessage : Type}
-    (T : Transcript pSpec) (dir : Direction) (msg : NextMessage) :
-        Transcript (pSpec ++ₚ .mkSingle dir NextMessage) :=
-  Transcript.append T fun _ => msg
-
-end Composition
-
 section Execution
 
 variable {n : ℕ} {pSpec : ProtocolSpec n} {ι : Type} {oSpec : OracleSpec ι}
@@ -384,11 +301,12 @@ def runProverAux [DecidableEq ι] [∀ i, Sampleable (pSpec.Challenge i)]
       OracleComp (oSpec ++ₒ challengeOracle pSpec)
         (PartialTranscript pSpec i × QueryLog oSpec × PrvState) := by
   induction i using Fin.induction with
-  | zero => simp; exact
+  | zero => exact
     (do
-      let ⟨state, queryLog⟩ ← liftComp (simulate loggingOracle ∅ <| pure (prover.load stmt wit))
-      return ⟨emptyPartialTranscript, queryLog, state⟩)
-  | succ j ih => simp [ProtocolSpec.take] at ih ⊢; exact
+      -- let ⟨state, queryLog⟩ ← liftComp (simulate loggingOracle ∅ <| pure (prover.load stmt wit))
+      letI state := prover.load stmt wit
+      return ⟨emptyPartialTranscript, ∅, state⟩)
+  | succ j ih => exact
     (do
       let ⟨transcript, queryLog, state⟩ ← ih
       match hDir : pSpec.getDir j with
@@ -396,12 +314,12 @@ def runProverAux [DecidableEq ι] [∀ i, Sampleable (pSpec.Challenge i)]
         let challenge ← query (Sum.inr ⟨j, hDir⟩) ()
         haveI challenge : pSpec.Challenge ⟨j, hDir⟩ := by simpa only
         letI newState := prover.receiveChallenge ⟨j, hDir⟩ state challenge
-        letI newTranscript := transcript.snoc (by omega) challenge
+        letI newTranscript := transcript.snoc (by simp) challenge
         return ⟨newTranscript, queryLog, newState⟩
       | .P_to_V => do
         let ⟨⟨msg, newState⟩, newQueryLog⟩ ← liftComp
           (simulate loggingOracle queryLog (prover.sendMessage ⟨j, hDir⟩ state))
-        letI newTranscript := transcript.snoc (by omega) msg
+        letI newTranscript := transcript.snoc (by simp) msg
         return ⟨newTranscript, newQueryLog, newState⟩
       )
 
